src/Std/Experimental/Do/WP/Lemmas.lean
@@ -21,79 +21,79 @@ Some lemmas prove only one direction (`⊑`) instead of equality because our `wp
 only provides one direction.
 -/
 
-namespace Std.Experimental.Do.WP
+namespace Std.Experimental.Do.WPMonad
 
-open Lean.Order WP
+open Lean.Order WPMonad
 
 universe u v
 variable {m : Type u → Type v}
 
 /-! ## MonadReaderOf simp lemmas -/
 
-theorem read_ReaderT_wp [Monad m] [Assertion Pred] [Assertion EPred] [WP m Pred EPred]
+theorem read_ReaderT_wp [Monad m] [Assertion Pred] [Assertion EPred] [WPMonad m Pred EPred]
     (post : ρ → ρ → Pred) (epost : EPred) :
     (fun r => post r r) ⊑ wp (MonadReaderOf.read : ReaderT ρ m ρ) post epost := by
   intro r
   simpa [MonadReaderOf.read] using
-    (WP.wp_pure (m := m) (x := r) (post := fun a => post a r) (epost := epost))
+    (WPMonad.wp_pure (m := m) (x := r) (post := fun a => post a r) (epost := epost))
 
 @[simp]
-theorem adapt_ReaderT_wp [Monad m] [Assertion Pred] [Assertion EPred] [WP m Pred EPred] (f : ρ → ρ') (x : ReaderT ρ' m α) :
+theorem adapt_ReaderT_wp [Monad m] [Assertion Pred] [Assertion EPred] [WPMonad m Pred EPred] (f : ρ → ρ') (x : ReaderT ρ' m α) :
     wp (ReaderT.adapt f x : ReaderT ρ m α) post epost =
       fun r => wp x (fun a _ => post a r) epost (f r) := rfl
 
 /-! ## MonadStateOf simp lemmas -/
 
-theorem get_StateT_wp [Monad m] [Assertion Pred] [Assertion EPred] [WP m Pred EPred]
+theorem get_StateT_wp [Monad m] [Assertion Pred] [Assertion EPred] [WPMonad m Pred EPred]
     (post : σ → σ → Pred) (epost : EPred) :
     (fun s => post s s) ⊑ wp (MonadStateOf.get : StateT σ m σ) post epost := by
   intro s
   simpa [MonadStateOf.get] using
-    (WP.wp_pure (m := m) (x := (s, s))
+    (WPMonad.wp_pure (m := m) (x := (s, s))
       (post := fun x => post x.fst x.snd) (epost := epost))
 
-theorem set_StateT_wp [Monad m] [Assertion Pred] [Assertion EPred] [WP m Pred EPred] (x : σ)
+theorem set_StateT_wp [Monad m] [Assertion Pred] [Assertion EPred] [WPMonad m Pred EPred] (x : σ)
     (post : PUnit → σ → Pred) (epost : EPred) :
     (fun _ => post ⟨⟩ x) ⊑ wp (MonadStateOf.set x : StateT σ m PUnit) post epost := by
   intro s
   simpa [MonadStateOf.set] using
-    (WP.wp_pure (m := m) (x := (PUnit.unit, x))
+    (WPMonad.wp_pure (m := m) (x := (PUnit.unit, x))
       (post := fun x => post x.fst x.snd) (epost := epost))
 
-theorem modifyGet_StateT_wp [Monad m] [Assertion Pred] [Assertion EPred] [WP m Pred EPred] (f : σ → α × σ)
+theorem modifyGet_StateT_wp [Monad m] [Assertion Pred] [Assertion EPred] [WPMonad m Pred EPred] (f : σ → α × σ)
     (post : α → σ → Pred) (epost : EPred) :
     (fun s => post (f s).1 (f s).2) ⊑ wp (MonadStateOf.modifyGet f : StateT σ m α) post epost := by
   intro s
   simpa [MonadStateOf.modifyGet] using
-    (WP.wp_pure (m := m) (x := f s)
+    (WPMonad.wp_pure (m := m) (x := f s)
       (post := fun x => post x.fst x.snd) (epost := epost))
 
 @[simp]
 theorem get_EStateM_wp :
     wp (MonadStateOf.get : EStateM ε σ σ) post epost = fun s => post s s := by
   funext s
-  simp only [wp, WP.wpTrans, MonadStateOf.get, EStateM.get]
+  simp only [wp, WPMonad.wpTrans, MonadStateOf.get, EStateM.get]
 
 @[simp]
 theorem set_EStateM_wp (x : σ) :
     wp (MonadStateOf.set x : EStateM ε σ PUnit) post epost = fun _ => post ⟨⟩ x := by
   funext s
-  simp only [wp, WP.wpTrans, MonadStateOf.set, EStateM.set]
+  simp only [wp, WPMonad.wpTrans, MonadStateOf.set, EStateM.set]
 
 @[simp]
 theorem modifyGet_EStateM_wp (f : σ → α × σ) :
     wp (MonadStateOf.modifyGet f : EStateM ε σ α) post epost = fun s => post (f s).1 (f s).2 := by
   funext s
-  simp only [wp, WP.wpTrans, MonadStateOf.modifyGet, EStateM.modifyGet]
+  simp only [wp, WPMonad.wpTrans, MonadStateOf.modifyGet, EStateM.modifyGet]
 
 @[simp]
-theorem modify_StateT_wp [Monad m] [Assertion Pred] [Assertion EPred] [WP m Pred EPred] (f : σ → σ) :
+theorem modify_StateT_wp [Monad m] [Assertion Pred] [Assertion EPred] [WPMonad m Pred EPred] (f : σ → σ) :
     wp (modify f : StateT σ m PUnit) post epost =
       wp (MonadStateOf.modifyGet fun s => (⟨⟩, f s) : StateT σ m PUnit) post epost := by
   rfl
 
 @[simp]
-theorem getModify_StateT_wp [Monad m] [Assertion Pred] [Assertion EPred] [WP m Pred EPred] (f : σ → σ) :
+theorem getModify_StateT_wp [Monad m] [Assertion Pred] [Assertion EPred] [WPMonad m Pred EPred] (f : σ → σ) :
     wp (getModify f : StateT σ m σ) post epost =
       wp (MonadStateOf.modifyGet fun s => (s, f s) : StateT σ m σ) post epost := by
   rfl
@@ -113,7 +113,7 @@ theorem getModify_EStateM_wp (f : σ → σ) :
 /-! ## MonadExceptOf simp lemmas -/
 
 @[simp]
-theorem throwThe_wp [MonadExceptOf ε m] [Monad m] [Assertion Pred] [Assertion EPred] [WP m Pred EPred] (err : ε) :
+theorem throwThe_wp [MonadExceptOf ε m] [Monad m] [Assertion Pred] [Assertion EPred] [WPMonad m Pred EPred] (err : ε) :
     wp (throwThe ε err : m α) post epost =
       wp (MonadExceptOf.throw err : m α) post epost := by
   rfl
@@ -121,19 +121,19 @@ theorem throwThe_wp [MonadExceptOf ε m] [Monad m] [Assertion Pred] [Assertion E
 @[simp]
 theorem throw_Except_wp (e : ε) :
     wp (MonadExceptOf.throw e : Except ε α) post epost = epost.head e := by
-  simp [wp, WP.wpTrans]
+  simp [wp, WPMonad.wpTrans]
 
-theorem throw_ExceptT_wp [Monad m] [Assertion Pred] [Assertion EPred] [WP m Pred EPred] (err : ε) :
+theorem throw_ExceptT_wp [Monad m] [Assertion Pred] [Assertion EPred] [WPMonad m Pred EPred] (err : ε) :
     epost.head err ⊑ wp (MonadExceptOf.throw err : ExceptT ε m α) post epost := by
   simpa [MonadExceptOf.throw, EPost.cons.pushExcept] using
-    (WP.wp_pure (m := m) (x := Except.error err)
+    (WPMonad.wp_pure (m := m) (x := Except.error err)
       (post := epost.pushExcept post) (epost := epost.tail))
 
 @[simp]
 theorem throw_EStateM_wp (e : ε) :
     wp (MonadExceptOf.throw e : EStateM ε σ α) post epost = epost e := by
   funext s
-  simp only [wp, WP.wpTrans, MonadExceptOf.throw, EStateM.throw]
+  simp only [wp, WPMonad.wpTrans, MonadExceptOf.throw, EStateM.throw]
 
 @[simp]
 theorem throw_Option_wp (e : PUnit) :
@@ -141,22 +141,22 @@ theorem throw_Option_wp (e : PUnit) :
   simp only [wp, MonadExceptOf.throw]
   rfl
 
-theorem throw_OptionT_wp [Monad m] [Assertion Pred] [Assertion EPred] [WP m Pred EPred] (err : PUnit) :
+theorem throw_OptionT_wp [Monad m] [Assertion Pred] [Assertion EPred] [WPMonad m Pred EPred] (err : PUnit) :
   epost.head ⊑ wp (MonadExceptOf.throw err : OptionT m α) post epost := by
   show epost.head ⊑ wp (pure none : m (Option α)) (epost.pushOption post) epost.tail
   simpa [MonadExceptOf.throw, EPost.cons.pushOption] using
-    (WP.wp_pure (m := m) (x := none)
+    (WPMonad.wp_pure (m := m) (x := none)
       (post := epost.pushOption post) (epost := epost.tail))
 
 @[simp]
-theorem tryCatch_MonadExcept_wp [MonadExceptOf ε m] [Monad m] [Assertion Pred] [Assertion EPred] [WP m Pred EPred] (x : m α)
+theorem tryCatch_MonadExcept_wp [MonadExceptOf ε m] [Monad m] [Assertion Pred] [Assertion EPred] [WPMonad m Pred EPred] (x : m α)
     (h : ε → m α) :
     wp (tryCatch x h : m α) post epost =
       wp (MonadExceptOf.tryCatch x h : m α) post epost := by
   rfl
 
 @[simp]
-theorem tryCatchThe_wp [MonadExceptOf ε m] [Monad m] [Assertion Pred] [Assertion EPred] [WP m Pred EPred] (x : m α) (h : ε → m α) :
+theorem tryCatchThe_wp [MonadExceptOf ε m] [Monad m] [Assertion Pred] [Assertion EPred] [WPMonad m Pred EPred] (x : m α) (h : ε → m α) :
     wp (tryCatchThe ε x h : m α) post epost =
       wp (MonadExceptOf.tryCatch x h : m α) post epost := by
   rfl
@@ -165,7 +165,7 @@ theorem tryCatchThe_wp [MonadExceptOf ε m] [Monad m] [Assertion Pred] [Assertio
 theorem tryCatch_Except_wp (x : Except ε α) (h : ε → Except ε α) :
     wp (MonadExceptOf.tryCatch x h : Except ε α) post epost =
       wp x post epost⟨fun e => wp (h e) post epost⟩ := by
-  simp only [wp, WP.wpTrans, MonadExceptOf.tryCatch, Except.tryCatch]
+  simp only [wp, WPMonad.wpTrans, MonadExceptOf.tryCatch, Except.tryCatch]
   cases x <;> simp
 
 -- TODO: Upstream
@@ -180,24 +180,24 @@ theorem tryCatch_Except_wp (x : Except ε α) (h : ε → Except ε α) :
   simp only [tryCatch, tryCatchThe, MonadExceptOf.tryCatch, ExceptT.tryCatch, ExceptT.run_mk]
   rfl
 
-theorem tryCatch_ExceptT_wp [Monad m] [Assertion Pred] [Assertion EPred] [WP m Pred EPred] (x : ExceptT ε m α)
+theorem tryCatch_ExceptT_wp [Monad m] [Assertion Pred] [Assertion EPred] [WPMonad m Pred EPred] (x : ExceptT ε m α)
     (h : ε → ExceptT ε m α) :
     wp x post ⟨fun e => wp (h e) post epost, epost.tail⟩ ⊑
       wp (MonadExceptOf.tryCatch x h : ExceptT ε m α) post epost := by
   change _ ⊑ wp (tryCatch x h : ExceptT ε m α) _ _
   simp only [ExceptT.apply_wp, ExceptT.run_tryCatch]
-  apply PartialOrder.rel_trans; rotate_left; apply WP.wp_bind
-  apply WP.wp_consequence; intro r; cases r with
+  apply PartialOrder.rel_trans; rotate_left; apply WPMonad.wp_bind
+  apply WPMonad.wp_consequence; intro r; cases r with
   | ok a =>
     simp; apply PartialOrder.rel_trans; rotate_left;
-    apply WP.wp_pure; simp; rfl
+    apply WPMonad.wp_pure; simp; rfl
   | error _ => exact PartialOrder.rel_refl
 
 @[simp]
 theorem tryCatch_Option_wp (x : Option α) (h : PUnit → Option α) :
   wp (MonadExceptOf.tryCatch x h : Option α) post epost =
     wp x post (wp (h ⟨⟩) post epost) := by
-  simp only [wp, WP.wpTrans, MonadExceptOf.tryCatch, Option.tryCatch]
+  simp only [wp, WPMonad.wpTrans, MonadExceptOf.tryCatch, Option.tryCatch]
   cases x <;> rfl
 
 
@@ -205,133 +205,133 @@ theorem tryCatch_EStateM_wp (x : EStateM ε σ α) (h : ε → EStateM ε σ α)
     wp (MonadExceptOf.tryCatch x h : EStateM ε σ α) post epost =
       fun s => wp x post (fun e s' => wp (h e) post epost s') s := by
   funext s
-  simp only [wp, WP.wpTrans, MonadExceptOf.tryCatch, EStateM.tryCatch]
+  simp only [wp, WPMonad.wpTrans, MonadExceptOf.tryCatch, EStateM.tryCatch]
   cases (x s) <;> simp
   rfl
 
 @[simp]
-theorem tryCatch_OptionT_wp [Monad m] [Assertion Pred] [Assertion EPred] [WP m Pred EPred] (x : OptionT m α)
+theorem tryCatch_OptionT_wp [Monad m] [Assertion Pred] [Assertion EPred] [WPMonad m Pred EPred] (x : OptionT m α)
     (h : PUnit → OptionT m α) :
   wp x post ⟨wp (h ⟨⟩) post epost, epost.tail⟩ ⊑
     wp (MonadExceptOf.tryCatch x h : OptionT m α) post epost := by
   simp only [wp, MonadExceptOf.tryCatch, OptionT.tryCatch, OptionT.mk, OptionT.run]
-  apply PartialOrder.rel_trans; rotate_left; apply WP.wp_bind
-  apply WP.wp_consequence (m := m); intro o; cases o with
+  apply PartialOrder.rel_trans; rotate_left; apply WPMonad.wp_bind
+  apply WPMonad.wp_consequence (m := m); intro o; cases o with
   | some a =>
-    apply PartialOrder.rel_trans; rotate_left; apply WP.wp_pure
+    apply PartialOrder.rel_trans; rotate_left; apply WPMonad.wp_pure
     simp [EPost.cons.pushOption]; exact PartialOrder.rel_refl
   | none => exact PartialOrder.rel_refl
 
 /-! ## Additional state operation lemmas -/
 
 @[simp]
-theorem getThe_StateT_wp [Monad m] [Assertion Pred] [Assertion EPred] [WP m Pred EPred] :
+theorem getThe_StateT_wp [Monad m] [Assertion Pred] [Assertion EPred] [WPMonad m Pred EPred] :
     wp (getThe σ : StateT σ m σ) post epost =
       wp (MonadStateOf.get : StateT σ m σ) post epost := by
   rfl
 
 @[simp]
-theorem modifyThe_StateT_wp [Monad m] [Assertion Pred] [Assertion EPred] [WP m Pred EPred] (f : σ → σ) :
+theorem modifyThe_StateT_wp [Monad m] [Assertion Pred] [Assertion EPred] [WPMonad m Pred EPred] (f : σ → σ) :
     wp (modifyThe σ f : StateT σ m PUnit) post epost =
       wp (MonadStateOf.modifyGet fun s => (⟨⟩, f s) : StateT σ m PUnit) post epost := by
   rfl
 
 @[simp]
-theorem modifyGetThe_StateT_wp [Monad m] [Assertion Pred] [Assertion EPred] [WP m Pred EPred] (f : σ → α × σ) :
+theorem modifyGetThe_StateT_wp [Monad m] [Assertion Pred] [Assertion EPred] [WPMonad m Pred EPred] (f : σ → α × σ) :
     wp (modifyGetThe σ f : StateT σ m α) post epost =
       wp (MonadStateOf.modifyGet f : StateT σ m α) post epost := by
   rfl
 
 @[simp]
-theorem get_MonadState_wp [Monad m] [Assertion Pred] [Assertion EPred] [WP m Pred EPred] [MonadStateOf σ m] :
+theorem get_MonadState_wp [Monad m] [Assertion Pred] [Assertion EPred] [WPMonad m Pred EPred] [MonadStateOf σ m] :
     wp (MonadState.get : m σ) post epost =
       wp (MonadStateOf.get : m σ) post epost := by
   rfl
 
 @[simp]
-theorem set_MonadState_wp [Monad m] [Assertion Pred] [Assertion EPred] [WP m Pred EPred] [MonadStateOf σ m] (x : σ) :
+theorem set_MonadState_wp [Monad m] [Assertion Pred] [Assertion EPred] [WPMonad m Pred EPred] [MonadStateOf σ m] (x : σ) :
     wp (MonadState.set x : m PUnit) post epost =
       wp (MonadStateOf.set x : m PUnit) post epost := by
   rfl
 
 @[simp]
-theorem modifyGet_MonadState_wp [Monad m] [Assertion Pred] [Assertion EPred] [WP m Pred EPred] [MonadStateOf σ m] (f : σ → α × σ) :
+theorem modifyGet_MonadState_wp [Monad m] [Assertion Pred] [Assertion EPred] [WPMonad m Pred EPred] [MonadStateOf σ m] (f : σ → α × σ) :
     wp (MonadState.modifyGet f : m α) post epost =
       wp (MonadStateOf.modifyGet f : m α) post epost := by
   rfl
 
 @[simp]
-theorem read_MonadReader_wp [Monad m] [Assertion Pred] [Assertion EPred] [WP m Pred EPred] [MonadReaderOf ρ m] :
+theorem read_MonadReader_wp [Monad m] [Assertion Pred] [Assertion EPred] [WPMonad m Pred EPred] [MonadReaderOf ρ m] :
     wp (MonadReader.read : m ρ) post epost =
       wp (MonadReaderOf.read : m ρ) post epost := by
   rfl
 
 @[simp]
-theorem readThe_ReaderT_wp [Monad m] [Assertion Pred] [Assertion EPred] [WP m Pred EPred] :
+theorem readThe_ReaderT_wp [Monad m] [Assertion Pred] [Assertion EPred] [WPMonad m Pred EPred] :
     wp (readThe ρ : ReaderT ρ m ρ) post epost =
       wp (MonadReaderOf.read : ReaderT ρ m ρ) post epost := by
   rfl
 
 /-! ## MonadLift simp lemmas -/
 
-theorem monadLift_StateT_wp [Monad m] [Assertion Pred] [Assertion EPred] [WP m Pred EPred] (x : m α) (post : α → σ → Pred) :
+theorem monadLift_StateT_wp [Monad m] [Assertion Pred] [Assertion EPred] [WPMonad m Pred EPred] (x : m α) (post : α → σ → Pred) :
     (fun s => wp x (fun a => post a s) epost) ⊑
       wp (MonadLift.monadLift x : StateT σ m α) post epost := by
   intro s
   simp only [wp, MonadLift.monadLift]
-  apply PartialOrder.rel_trans; rotate_left; apply WP.wp_bind
-  apply WP.wp_consequence (m := m); intro a
+  apply PartialOrder.rel_trans; rotate_left; apply WPMonad.wp_bind
+  apply WPMonad.wp_consequence (m := m); intro a
   simpa using
-    (WP.wp_pure (m := m) (x := (a, s))
+    (WPMonad.wp_pure (m := m) (x := (a, s))
       (post := fun x => post x.fst x.snd) (epost := epost))
 
 @[simp]
-theorem monadLift_ReaderT_wp [Monad m] [Assertion Pred] [Assertion EPred] [WP m Pred EPred] (x : m α) :
+theorem monadLift_ReaderT_wp [Monad m] [Assertion Pred] [Assertion EPred] [WPMonad m Pred EPred] (x : m α) :
     wp (MonadLift.monadLift x : ReaderT ρ m α) post epost =
       fun r => wp x (fun a => post a r) epost := by
   rfl
 
-theorem monadLift_ExceptT_wp [Monad m] [Assertion Pred] [Assertion EPred] [WP m Pred EPred] (x : m α) (post : α → Pred)
+theorem monadLift_ExceptT_wp [Monad m] [Assertion Pred] [Assertion EPred] [WPMonad m Pred EPred] (x : m α) (post : α → Pred)
     (epost : EPost.cons (ε → Pred) EPred) :
     wp x post epost.tail ⊑
       wp (MonadLift.monadLift x : ExceptT ε m α) post epost := by
   simp only [wp, MonadLift.monadLift, ExceptT.lift, ExceptT.mk]
   apply PartialOrder.rel_trans; rotate_left
-  · exact WP.wp_map (m := m) Except.ok x _ _
+  · exact WPMonad.wp_map (m := m) Except.ok x _ _
   · exact PartialOrder.rel_refl
 
 @[simp]
-theorem lift_StateT_wp [Monad m] [Assertion Pred] [Assertion EPred] [WP m Pred EPred] (x : m α) :
+theorem lift_StateT_wp [Monad m] [Assertion Pred] [Assertion EPred] [WPMonad m Pred EPred] (x : m α) :
     wp (StateT.lift x : StateT σ m α) post epost =
       wp (MonadLift.monadLift x : StateT σ m α) post epost := by
   rfl
 
 @[simp]
-theorem lift_ExceptT_wp [Monad m] [Assertion Pred] [Assertion EPred] [WP m Pred EPred] (x : m α) :
+theorem lift_ExceptT_wp [Monad m] [Assertion Pred] [Assertion EPred] [WPMonad m Pred EPred] (x : m α) :
     wp (ExceptT.lift x : ExceptT ε m α) post epost =
       wp (MonadLift.monadLift x : ExceptT ε m α) post epost := by
   rfl
 
 @[simp]
-theorem monadLift_OptionT_wp [Monad m] [Assertion Pred] [Assertion EPred] [WP m Pred EPred] (x : m α) :
+theorem monadLift_OptionT_wp [Monad m] [Assertion Pred] [Assertion EPred] [WPMonad m Pred EPred] (x : m α) :
   wp x post epost.tail ⊑
     wp (MonadLift.monadLift x : OptionT m α) post epost := by
   simp only [wp, MonadLift.monadLift, OptionT.mk, OptionT.lift, OptionT.run]
-  apply PartialOrder.rel_trans; rotate_left; apply WP.wp_bind
-  apply WP.wp_consequence (m := m); intro a
-  apply PartialOrder.rel_trans; rotate_left; apply WP.wp_pure
+  apply PartialOrder.rel_trans; rotate_left; apply WPMonad.wp_bind
+  apply WPMonad.wp_consequence (m := m); intro a
+  apply PartialOrder.rel_trans; rotate_left; apply WPMonad.wp_pure
   simp [EPost.cons.pushOption]; exact PartialOrder.rel_refl
 
 @[simp]
-theorem lift_OptionT_wp [Monad m] [Assertion Pred] [Assertion EPred] [WP m Pred EPred]
-    [Assertion (EPost.cons Pred EPred)] [WP (OptionT m) Pred (EPost.cons Pred EPred)] (x : m α) :
+theorem lift_OptionT_wp [Monad m] [Assertion Pred] [Assertion EPred] [WPMonad m Pred EPred]
+    [Assertion (EPost.cons Pred EPred)] [WPMonad (OptionT m) Pred (EPost.cons Pred EPred)] (x : m α) :
     wp (OptionT.lift x : OptionT m α) post epost =
       wp (MonadLift.monadLift x : OptionT m α) post epost := rfl
 
 /-! ## MonadFunctor simp lemmas -/
 
 @[simp]
-theorem monadMap_StateT_wp [Monad m] [Assertion Pred] [Assertion EPred] [WP m Pred EPred]
+theorem monadMap_StateT_wp [Monad m] [Assertion Pred] [Assertion EPred] [WPMonad m Pred EPred]
     (f : ∀{β}, m β → m β) {α} (x : StateT σ m α) (post : α → σ → Pred) (epost : EPred) :
     wp (MonadFunctor.monadMap (m:=m) f x : StateT σ m α) post epost =
       fun s => wp (f (x.run s)) (fun (a, s') => post a s') epost := by
@@ -339,7 +339,7 @@ theorem monadMap_StateT_wp [Monad m] [Assertion Pred] [Assertion EPred] [WP m Pr
   simp [MonadFunctor.monadMap, StateT.run]
 
 @[simp]
-theorem monadMap_ReaderT_wp [Monad m] [Assertion Pred] [Assertion EPred] [WP m Pred EPred]
+theorem monadMap_ReaderT_wp [Monad m] [Assertion Pred] [Assertion EPred] [WPMonad m Pred EPred]
     (f : ∀{β}, m β → m β) {α} (x : ReaderT ρ m α) (post : α → ρ → Pred) (epost : EPred) :
     wp (MonadFunctor.monadMap (m:=m) f x : ReaderT ρ m α) post epost =
       fun r => wp (f (x.run r)) (fun a => post a r) epost := by
@@ -347,7 +347,7 @@ theorem monadMap_ReaderT_wp [Monad m] [Assertion Pred] [Assertion EPred] [WP m P
   simp [MonadFunctor.monadMap, ReaderT.run]
 
 @[simp]
-theorem monadMap_ExceptT_wp [Monad m] [Assertion Pred] [Assertion EPred] [WP m Pred EPred]
+theorem monadMap_ExceptT_wp [Monad m] [Assertion Pred] [Assertion EPred] [WPMonad m Pred EPred]
     (f : ∀{β}, m β → m β) {α} (x : ExceptT ε m α) (post : α → Pred)
     (epost : EPost.cons (ε → Pred) EPred) :
     wp (MonadFunctor.monadMap (m:=m) f x : ExceptT ε m α) post epost =
@@ -355,57 +355,57 @@ theorem monadMap_ExceptT_wp [Monad m] [Assertion Pred] [Assertion EPred] [WP m P
   simp [MonadFunctor.monadMap, ExceptT.run]
 
 @[simp]
-theorem monadMap_OptionT_wp [Monad m] [Assertion Pred] [Assertion EPred] [WP m Pred EPred]
+theorem monadMap_OptionT_wp [Monad m] [Assertion Pred] [Assertion EPred] [WPMonad m Pred EPred]
   (f : ∀{β}, m β → m β) {α} (x : OptionT m α) (post : α → Pred) (epost : EPost.cons Pred EPred) :
   wp (MonadFunctor.monadMap (m:=m) f x : OptionT m α) post epost =
     wp (f x.run) (epost.pushOption post) epost.tail := by
   simp only [wp, MonadFunctor.monadMap, OptionT.run]; rfl
 
 @[simp]
-theorem withReader_ReaderT_wp [Monad m] [Assertion Pred] [Assertion EPred] [WP m Pred EPred] (f : ρ → ρ) (x : ReaderT ρ m α) :
+theorem withReader_ReaderT_wp [Monad m] [Assertion Pred] [Assertion EPred] [WPMonad m Pred EPred] (f : ρ → ρ) (x : ReaderT ρ m α) :
     wp (MonadWithReaderOf.withReader f x : ReaderT ρ m α) post epost =
       fun r => wp x (fun a _ => post a r) epost (f r) := rfl
 
 @[simp]
-theorem withReader_MonadWithReader_wp [Monad m] [Assertion Pred] [Assertion EPred] [WP m Pred EPred] [MonadWithReaderOf ρ m]
+theorem withReader_MonadWithReader_wp [Monad m] [Assertion Pred] [Assertion EPred] [WPMonad m Pred EPred] [MonadWithReaderOf ρ m]
     (f : ρ → ρ) (x : m α) :
     wp (MonadWithReader.withReader f x : m α) post epost =
       wp (MonadWithReaderOf.withReader f x : m α) post epost := rfl
 
 @[simp]
-theorem withTheReader_ReaderT_wp [Monad m] [Assertion Pred] [Assertion EPred] [WP m Pred EPred] (f : ρ → ρ) (x : ReaderT ρ m α) :
+theorem withTheReader_ReaderT_wp [Monad m] [Assertion Pred] [Assertion EPred] [WPMonad m Pred EPred] (f : ρ → ρ) (x : ReaderT ρ m α) :
     wp (withTheReader ρ f x : ReaderT ρ m α) post epost =
       wp (MonadWithReaderOf.withReader f x : ReaderT ρ m α) post epost := rfl
 
 /-! ## Transformer adapt lemmas -/
 
-theorem adapt_ExceptT_wp [Monad m] [Assertion Pred] [Assertion EPred] [WP m Pred EPred] (f : ε → ε') (x : ExceptT ε m α) :
+theorem adapt_ExceptT_wp [Monad m] [Assertion Pred] [Assertion EPred] [WPMonad m Pred EPred] (f : ε → ε') (x : ExceptT ε m α) :
     wp x post ⟨fun e => epost.head (f e), epost.tail⟩ ⊑
       wp (ExceptT.adapt f x : ExceptT ε' m α) post epost := by
   simp only [wp, ExceptT.adapt, ExceptT.mk]
   apply PartialOrder.rel_trans; rotate_left
-  · exact WP.wp_map (m := m) (Except.mapError f) x _ _
-  · apply WP.wp_consequence (m := m); intro r; cases r <;> exact PartialOrder.rel_refl
+  · exact WPMonad.wp_map (m := m) (Except.mapError f) x _ _
+  · apply WPMonad.wp_consequence (m := m); intro r; cases r <;> exact PartialOrder.rel_refl
 
 @[simp]
 theorem adaptExcept_EStateM_wp (f : ε → ε') (x : EStateM ε σ α) :
     wp (EStateM.adaptExcept f x : EStateM ε' σ α) post epost =
       wp x post (fun e => epost (f e)) := by
   funext s
-  simp only [wp, WP.wpTrans, EStateM.adaptExcept]
+  simp only [wp, WPMonad.wpTrans, EStateM.adaptExcept]
   cases (x s) <;> simp
 
 /-! ## MonadControl simp lemmas -/
 
 @[simp]
-theorem liftWith_StateT_wp [Monad m] [Assertion Pred] [Assertion EPred] [WP m Pred EPred]
+theorem liftWith_StateT_wp [Monad m] [Assertion Pred] [Assertion EPred] [WPMonad m Pred EPred]
     (f : (∀{β}, StateT σ m β → m (β × σ)) → m α) :
     wp (MonadControl.liftWith (m:=m) f : StateT σ m α) post epost s =
       wp ((fun a => (a, s)) <$> f (fun x => x.run s)) (fun ⟨a, s⟩ => post a s) epost := by
   simp [MonadControl.liftWith]
 
 @[simp]
-theorem liftWith_ReaderT_wp [Monad m] [Assertion Pred] [Assertion EPred] [WP m Pred EPred]
+theorem liftWith_ReaderT_wp [Monad m] [Assertion Pred] [Assertion EPred] [WPMonad m Pred EPred]
     (f : (∀{β}, ReaderT ρ m β → m β) → m α) :
     wp (MonadControl.liftWith (m:=m) f : ReaderT ρ m α) post epost r =
       wp (f (fun x => x.run r)) (fun a => post a r) epost := by
@@ -416,7 +416,7 @@ theorem liftWith_ReaderT_wp [Monad m] [Assertion Pred] [Assertion EPred] [WP m P
     (liftM x : ExceptT ε m α).run = (Except.ok <$> x : m (Except ε α)) := rfl
 
 @[simp]
-theorem liftWith_ExceptT_wp [Monad m] [Assertion Pred] [Assertion EPred] [WP m Pred EPred]
+theorem liftWith_ExceptT_wp [Monad m] [Assertion Pred] [Assertion EPred] [WPMonad m Pred EPred]
     (f : (∀{β}, ExceptT ε m β → m (Except ε β)) → m α) :
     wp (MonadControl.liftWith (m:=m) f : ExceptT ε m α) post epost =
       wp (Except.ok <$> f (fun x => x.run)) (epost.pushExcept post) epost.tail := by
@@ -425,59 +425,59 @@ theorem liftWith_ExceptT_wp [Monad m] [Assertion Pred] [Assertion EPred] [WP m P
   simp
 
 @[simp]
-theorem liftWith_OptionT_wp [Monad m] [Assertion Pred] [Assertion EPred] [WP m Pred EPred]
+theorem liftWith_OptionT_wp [Monad m] [Assertion Pred] [Assertion EPred] [WPMonad m Pred EPred]
   (f : (∀{β}, OptionT m β → m (Option β)) → m α) :
   wp (f (fun x => x.run)) post epost.tail ⊑
     wp (MonadControl.liftWith (m:=m) f : OptionT m α) post epost := by
   simp only [MonadControl.liftWith, liftM, monadLift, OptionT.apply_wp]
   exact monadLift_OptionT_wp (f (fun x => x.run))
 
-theorem restoreM_StateT_wp [Monad m] [Assertion Pred] [Assertion EPred] [WP m Pred EPred] (x : m (α × σ)) :
+theorem restoreM_StateT_wp [Monad m] [Assertion Pred] [Assertion EPred] [WPMonad m Pred EPred] (x : m (α × σ)) :
     (fun _ => wp x (fun (a, s) => post a s) epost) ⊑
       wp (MonadControl.restoreM (m:=m) x : StateT σ m α) post epost := by
   simp only [MonadControl.restoreM]
-  apply PartialOrder.rel_trans; rotate_left; apply WP.wp_bind; simp only [liftM, monadLift]
+  apply PartialOrder.rel_trans; rotate_left; apply WPMonad.wp_bind; simp only [liftM, monadLift]
   apply PartialOrder.rel_trans; rotate_left; apply monadLift_StateT_wp
-  intro s; apply WP.wp_consequence; intro s'; simp only
-  apply PartialOrder.rel_trans; rotate_left; apply WP.wp_bind
+  intro s; apply WPMonad.wp_consequence; intro s'; simp only
+  apply PartialOrder.rel_trans; rotate_left; apply WPMonad.wp_bind
   simp [set, StateT.set, pure, StateT.pure]
   apply PartialOrder.rel_trans
   · simpa using
-      (WP.wp_pure (m := m) (x := (s'.fst, s'.snd))
+      (WPMonad.wp_pure (m := m) (x := (s'.fst, s'.snd))
         (post := fun x => post x.fst x.snd) (epost := epost))
   · simpa using
-      (WP.wp_pure (m := m) (x := (PUnit.unit, s'.snd))
+      (WPMonad.wp_pure (m := m) (x := (PUnit.unit, s'.snd))
         (post := fun x => wp (pure (s'.fst, x.snd)) (fun x => post x.fst x.snd) epost)
         (epost := epost))
 
 @[simp]
-theorem restoreM_ReaderT_wp [Monad m] [Assertion Pred] [Assertion EPred] [WP m Pred EPred] (x : m α) :
+theorem restoreM_ReaderT_wp [Monad m] [Assertion Pred] [Assertion EPred] [WPMonad m Pred EPred] (x : m α) :
     wp (MonadControl.restoreM (m:=m) x : ReaderT ρ m α) post epost =
       fun r => wp x (fun a => post a r) epost := by
   funext r
   simp [MonadControl.restoreM, ReaderT.run]
 
 @[simp]
-theorem restoreM_ExceptT_wp [Monad m] [Assertion Pred] [Assertion EPred] [WP m Pred EPred] (x : m (Except ε α)) :
+theorem restoreM_ExceptT_wp [Monad m] [Assertion Pred] [Assertion EPred] [WPMonad m Pred EPred] (x : m (Except ε α)) :
     wp (MonadControl.restoreM (m:=m) x : ExceptT ε m α) post epost =
       wp x (epost.pushExcept post) epost.tail := by
   simp [MonadControl.restoreM, ExceptT.run]
 
 @[simp]
-theorem restoreM_OptionT_wp [Monad m] [Assertion Pred] [Assertion EPred] [WP m Pred EPred] (x : m (Option α)) :
+theorem restoreM_OptionT_wp [Monad m] [Assertion Pred] [Assertion EPred] [WPMonad m Pred EPred] (x : m (Option α)) :
   wp (MonadControl.restoreM (m:=m) x : OptionT m α) post epost =
     wp x (epost.pushOption post) epost.tail := by
   simp only [wp, MonadControl.restoreM]; rfl
 
 @[simp]
-theorem controlAt_wp [Bind n] [Monad n] [Monad m] [Assertion Pred] [Assertion EPred] [WP n Pred EPred] [MonadControlT m n]
+theorem controlAt_wp [Bind n] [Monad n] [Monad m] [Assertion Pred] [Assertion EPred] [WPMonad n Pred EPred] [MonadControlT m n]
     (f : (∀{β}, n β → m (stM m n β)) → m (stM m n α)) :
     wp (controlAt m f : n α) post epost =
       wp (liftWith f >>= restoreM : n α) post epost := by
   rfl
 
 @[simp]
-theorem control_wp [Bind n] [Monad n] [Monad m] [Assertion Pred] [Assertion EPred] [WP n Pred EPred] [MonadControlT m n]
+theorem control_wp [Bind n] [Monad n] [Monad m] [Assertion Pred] [Assertion EPred] [WPMonad n Pred EPred] [MonadControlT m n]
     (f : (∀{β}, n β → m (stM m n β)) → m (stM m n α)) :
     wp (control f : n α) post epost =
       wp (liftWith f >>= restoreM : n α) post epost := by
@@ -486,24 +486,24 @@ theorem control_wp [Bind n] [Monad n] [Monad m] [Assertion Pred] [Assertion EPre
 /-! ## Transitive lift/map simp lemmas -/
 
 @[simp]
-theorem monadLift_trans_wp [Monad o] [Assertion Pred] [Assertion EPred] [WP o Pred EPred] [MonadLift n o] [MonadLiftT m n] (x : m α) :
+theorem monadLift_trans_wp [Monad o] [Assertion Pred] [Assertion EPred] [WPMonad o Pred EPred] [MonadLift n o] [MonadLiftT m n] (x : m α) :
     wp (MonadLiftT.monadLift x : o α) post epost =
       wp (MonadLift.monadLift (m:=n) (MonadLiftT.monadLift (m:=m) x) : o α) post epost := rfl
 
 @[simp]
-theorem monadLift_refl_wp [Monad m] [Assertion Pred] [Assertion EPred] [WP m Pred EPred] [Pure m] (x : m α) :
+theorem monadLift_refl_wp [Monad m] [Assertion Pred] [Assertion EPred] [WPMonad m Pred EPred] [Pure m] (x : m α) :
     wp (MonadLiftT.monadLift x : m α) post epost =
       wp (x : m α) post epost := rfl
 
 @[simp]
-theorem monadMap_trans_wp [Monad o] [Assertion Pred] [Assertion EPred] [WP o Pred EPred] [MonadFunctor n o] [MonadFunctorT m n]
+theorem monadMap_trans_wp [Monad o] [Assertion Pred] [Assertion EPred] [WPMonad o Pred EPred] [MonadFunctor n o] [MonadFunctorT m n]
     (x : o α) :
     wp (MonadFunctorT.monadMap f x : o α) post epost =
       wp (MonadFunctor.monadMap (m:=n) (MonadFunctorT.monadMap (m:=m) f) x : o α) post epost := by
   rfl
 
 @[simp]
-theorem monadMap_refl_wp [Monad m] [Assertion Pred] [Assertion EPred] [WP m Pred EPred] [Pure m] (x : m α) :
+theorem monadMap_refl_wp [Monad m] [Assertion Pred] [Assertion EPred] [WPMonad m Pred EPred] [Pure m] (x : m α) :
     wp (MonadFunctorT.monadMap f x : m α) post epost =
       wp (f x : m α) post epost := by rfl
 
@@ -511,48 +511,48 @@ theorem monadMap_refl_wp [Monad m] [Assertion Pred] [Assertion EPred] [WP m Pred
 
 @[simp]
 theorem get_MonadStateOf_lift_wp [MonadStateOf σ m] [MonadLift m n] [Monad m] [Monad n]
-    [Assertion Pred] [Assertion EPred'] [WP n Pred EPred'] :
+    [Assertion Pred] [Assertion EPred'] [WPMonad n Pred EPred'] :
     wp (MonadStateOf.get : n σ) post epost =
       wp (MonadLift.monadLift (MonadStateOf.get : m σ) : n σ) post epost := by
   rfl
 
 @[simp]
 theorem set_MonadStateOf_lift_wp [MonadStateOf σ m] [MonadLift m n] [Monad m] [Monad n]
-    [Assertion Pred] [Assertion EPred'] [WP n Pred EPred'] (x : σ) :
+    [Assertion Pred] [Assertion EPred'] [WPMonad n Pred EPred'] (x : σ) :
     wp (MonadStateOf.set x : n PUnit) post epost =
       wp (MonadLift.monadLift (MonadStateOf.set (σ:=σ) x : m PUnit) : n PUnit) post epost := by
   rfl
 
 @[simp]
 theorem modifyGet_MonadStateOf_lift_wp [MonadStateOf σ m] [MonadLift m n] [Monad m] [Monad n]
-    [Assertion Pred] [Assertion EPred'] [WP n Pred EPred'] (f : σ → α × σ) :
+    [Assertion Pred] [Assertion EPred'] [WPMonad n Pred EPred'] (f : σ → α × σ) :
     wp (MonadStateOf.modifyGet f : n α) post epost =
       wp (MonadLift.monadLift (MonadState.modifyGet f : m α) : n α) post epost := by
   rfl
 
 @[simp]
 theorem read_MonadReaderOf_lift_wp [MonadReaderOf ρ m] [MonadLift m n] [Monad m] [Monad n]
-    [Assertion Pred] [Assertion EPred'] [WP n Pred EPred'] :
+    [Assertion Pred] [Assertion EPred'] [WPMonad n Pred EPred'] :
     wp (MonadReaderOf.read : n ρ) post epost =
       wp (MonadLift.monadLift (MonadReader.read : m ρ) : n ρ) post epost := by
   rfl
 
 @[simp]
-theorem throw_lift_ExceptT_wp [Monad m] [LawfulMonad m] [Assertion Pred] [Assertion EPred'] [WP m Pred EPred'] [MonadExceptOf ε m]
+theorem throw_lift_ExceptT_wp [Monad m] [LawfulMonad m] [Assertion Pred] [Assertion EPred'] [WPMonad m Pred EPred'] [MonadExceptOf ε m]
     (err : ε) :
     wp (MonadExceptOf.throw (ε:=ε) err : ExceptT ε' m α) post epost =
       wp (MonadExceptOf.throw (ε:=ε) err : m (Except ε' α)) (epost.pushExcept post) epost.tail := by
   rfl
 
 @[simp]
-theorem throw_lift_OptionT_wp [Monad m] [LawfulMonad m] [Assertion Pred] [Assertion EPred'] [WP m Pred EPred']
+theorem throw_lift_OptionT_wp [Monad m] [LawfulMonad m] [Assertion Pred] [Assertion EPred'] [WPMonad m Pred EPred']
     [MonadExceptOf ε m] (err : ε) :
   wp (MonadExceptOf.throw (ε:=ε) err : OptionT m α) post epost =
     wp (MonadExceptOf.throw (ε:=ε) err : m (Option α)) (epost.pushOption post) epost.tail := by
   rfl
 
 @[simp]
-theorem tryCatch_lift_ExceptT_wp [Monad m] [LawfulMonad m] [Assertion Pred] [Assertion EPred'] [WP m Pred EPred'] [MonadExceptOf ε m]
+theorem tryCatch_lift_ExceptT_wp [Monad m] [LawfulMonad m] [Assertion Pred] [Assertion EPred'] [WPMonad m Pred EPred'] [MonadExceptOf ε m]
     (x : ExceptT ε' m α) (h : ε → ExceptT ε' m α) :
     wp (MonadExceptOf.tryCatch (ε:=ε) x h : ExceptT ε' m α) post epost =
       wp (MonadExceptOf.tryCatch (ε:=ε) x h : m (Except ε' α))
@@ -560,7 +560,7 @@ theorem tryCatch_lift_ExceptT_wp [Monad m] [LawfulMonad m] [Assertion Pred] [Ass
   rfl
 
 @[simp]
-theorem tryCatch_lift_OptionT_wp [Monad m] [LawfulMonad m] [Assertion Pred] [Assertion EPred'] [WP m Pred EPred']
+theorem tryCatch_lift_OptionT_wp [Monad m] [LawfulMonad m] [Assertion Pred] [Assertion EPred'] [WPMonad m Pred EPred']
     [MonadExceptOf ε m] (x : OptionT m α) (h : ε → OptionT m α) :
   wp (MonadExceptOf.tryCatch (ε:=ε) x h : OptionT m α) post epost =
     wp (MonadExceptOf.tryCatch (ε:=ε) x h : m (Option α))
@@ -568,7 +568,7 @@ theorem tryCatch_lift_OptionT_wp [Monad m] [LawfulMonad m] [Assertion Pred] [Ass
   rfl
 
 @[simp]
-theorem throw_ReaderT_lift_wp [Monad m] [LawfulMonad m] [Assertion Pred] [Assertion EPred'] [WP m Pred EPred'] [MonadExceptOf ε m]
+theorem throw_ReaderT_lift_wp [Monad m] [LawfulMonad m] [Assertion Pred] [Assertion EPred'] [WPMonad m Pred EPred'] [MonadExceptOf ε m]
     (err : ε) :
     wp (MonadExceptOf.throw (ε:=ε) err : ReaderT ρ m α) post epost =
       wp (MonadLift.monadLift (MonadExceptOf.throw (ε:=ε) err : m α) :
@@ -576,7 +576,7 @@ theorem throw_ReaderT_lift_wp [Monad m] [LawfulMonad m] [Assertion Pred] [Assert
   rfl
 
 @[simp]
-theorem throw_StateT_lift_wp [Monad m] [LawfulMonad m] [Assertion Pred] [Assertion EPred'] [WP m Pred EPred'] [MonadExceptOf ε m]
+theorem throw_StateT_lift_wp [Monad m] [LawfulMonad m] [Assertion Pred] [Assertion EPred'] [WPMonad m Pred EPred'] [MonadExceptOf ε m]
     (err : ε) :
     wp (MonadExceptOf.throw (ε:=ε) err : StateT σ m α) post epost =
       wp (MonadLift.monadLift (MonadExceptOf.throw (ε:=ε) err : m α) :
@@ -584,7 +584,7 @@ theorem throw_StateT_lift_wp [Monad m] [LawfulMonad m] [Assertion Pred] [Asserti
   rfl
 
 @[simp]
-theorem tryCatch_ReaderT_lift_wp [Monad m] [LawfulMonad m] [Assertion Pred] [Assertion EPred'] [WP m Pred EPred'] [MonadExceptOf ε m]
+theorem tryCatch_ReaderT_lift_wp [Monad m] [LawfulMonad m] [Assertion Pred] [Assertion EPred'] [WPMonad m Pred EPred'] [MonadExceptOf ε m]
     (x : ReaderT ρ m α) (h : ε → ReaderT ρ m α) :
     wp (MonadExceptOf.tryCatch (ε:=ε) x h : ReaderT ρ m α) post epost =
       fun r => wp (MonadExceptOf.tryCatch (ε:=ε) (x.run r) (fun e => (h e).run r) : m α)
@@ -592,7 +592,7 @@ theorem tryCatch_ReaderT_lift_wp [Monad m] [LawfulMonad m] [Assertion Pred] [Ass
   rfl
 
 @[simp]
-theorem tryCatch_StateT_lift_wp [Monad m] [LawfulMonad m] [Assertion Pred] [Assertion EPred'] [WP m Pred EPred'] [MonadExceptOf ε m]
+theorem tryCatch_StateT_lift_wp [Monad m] [LawfulMonad m] [Assertion Pred] [Assertion EPred'] [WPMonad m Pred EPred'] [MonadExceptOf ε m]
     (x : StateT σ m α) (h : ε → StateT σ m α) :
     wp (MonadExceptOf.tryCatch (ε:=ε) x h : StateT σ m α) post epost =
       fun s => wp (MonadExceptOf.tryCatch (ε:=ε) (x.run s) (fun e => (h e).run s) : m (α × σ))
@@ -602,7 +602,7 @@ theorem tryCatch_StateT_lift_wp [Monad m] [LawfulMonad m] [Assertion Pred] [Asse
 /-! ## Transitive MonadControl lemmas -/
 
 @[simp]
-theorem liftWith_trans_wp [Monad o] [Assertion Pred] [Assertion EPred] [WP o Pred EPred] [MonadControl n o] [MonadControlT m n]
+theorem liftWith_trans_wp [Monad o] [Assertion Pred] [Assertion EPred] [WPMonad o Pred EPred] [MonadControl n o] [MonadControlT m n]
     (f : (∀{β}, o β → m (stM m o β)) → m α) :
     wp (MonadControlT.liftWith f : o α) post epost =
       wp (MonadControl.liftWith (m:=n) fun x₂ =>
@@ -610,14 +610,14 @@ theorem liftWith_trans_wp [Monad o] [Assertion Pred] [Assertion EPred] [WP o Pre
   rfl
 
 @[simp]
-theorem liftWith_refl_wp [Pure m] [Monad m] [Assertion Pred] [Assertion EPred] [WP m Pred EPred]
+theorem liftWith_refl_wp [Pure m] [Monad m] [Assertion Pred] [Assertion EPred] [WPMonad m Pred EPred]
     (f : (∀{β}, m β → m β) → m α) :
     wp (MonadControlT.liftWith (m:=m) f : m α) post epost =
       wp (f (fun x => x) : m α) post epost := by
   rfl
 
 @[simp]
-theorem restoreM_trans_wp [Monad o] [Assertion Pred] [Assertion EPred] [WP o Pred EPred] [MonadControl n o] [MonadControlT m n]
+theorem restoreM_trans_wp [Monad o] [Assertion Pred] [Assertion EPred] [WPMonad o Pred EPred] [MonadControl n o] [MonadControlT m n]
     (x : stM m o α) :
     wp (MonadControlT.restoreM x : o α) post epost =
       wp (MonadControl.restoreM (m:=n) (MonadControlT.restoreM (m:=m) x) : o α)
@@ -625,7 +625,7 @@ theorem restoreM_trans_wp [Monad o] [Assertion Pred] [Assertion EPred] [WP o Pre
   rfl
 
 @[simp]
-theorem restoreM_refl_wp [Pure m] [Monad m] [Assertion Pred] [Assertion EPred] [WP m Pred EPred] (x : stM m m α) :
+theorem restoreM_refl_wp [Pure m] [Monad m] [Assertion Pred] [Assertion EPred] [WPMonad m Pred EPred] (x : stM m m α) :
     wp (MonadControlT.restoreM x : m α) post epost =
       wp (Pure.pure x : m α) post epost := by
   rfl
@@ -633,7 +633,7 @@ theorem restoreM_refl_wp [Pure m] [Monad m] [Assertion Pred] [Assertion EPred] [
 /-! ## OrElse simp lemmas -/
 
 @[simp]
-theorem orElse_Except_wp [Monad m] [Assertion Pred] [Assertion EPred] [WP m Pred EPred] (x : Except ε α) (h : Unit → Except ε α) :
+theorem orElse_Except_wp [Monad m] [Assertion Pred] [Assertion EPred] [WPMonad m Pred EPred] (x : Except ε α) (h : Unit → Except ε α) :
     wp (OrElse.orElse x h : Except ε α) post epost =
       wp x post epost⟨fun _ => wp (h ()) post epost⟩ := by
   simp only [wp, OrElse.orElse, MonadExcept.orElse]
@@ -649,7 +649,7 @@ theorem orElse_Except_wp [Monad m] [Assertion Pred] [Assertion EPred] [WP m Pred
       | .error _ => (h ()).run) := by
   simp [OrElse.orElse, MonadExcept.orElse]
 
-theorem orElse_ExceptT_wp [Monad m] [Assertion Pred] [Assertion EPred] [WP m Pred EPred] (x : ExceptT ε m α)
+theorem orElse_ExceptT_wp [Monad m] [Assertion Pred] [Assertion EPred] [WPMonad m Pred EPred] (x : ExceptT ε m α)
     (h : Unit → ExceptT ε m α) :
     wp x post ⟨fun _ => wp (h ()) post epost, epost.tail⟩ ⊑
       wp (OrElse.orElse x h : ExceptT ε m α) post epost := by
@@ -660,7 +660,7 @@ theorem orElse_Option_wp (x : Option α) (h : Unit → Option α) :
   ∀ post (epost : Prop),
   wp (OrElse.orElse x h : Option α) post epost =
     wp x post (wp (h ()) post epost) := by
-  simp only [wp, WP.wpTrans, OrElse.orElse, Option.orElse]
+  simp only [wp, WPMonad.wpTrans, OrElse.orElse, Option.orElse]
   cases x <;> intro _ _ <;> rfl
 
 @[simp]
@@ -668,20 +668,20 @@ theorem orElse_EStateM_wp (x : EStateM ε σ α) (h : Unit → EStateM ε σ α)
     wp (OrElse.orElse x h : EStateM ε σ α) post epost =
       fun s => wp x post (fun _ s' => wp (h ()) post epost s') s := by
   funext s
-  simp only [wp, WP.wpTrans, OrElse.orElse, EStateM.orElse]
+  simp only [wp, WPMonad.wpTrans, OrElse.orElse, EStateM.orElse]
   cases x s <;> simp; rfl
 
 @[simp]
-theorem orElse_OptionT_wp [Monad m] [Assertion Pred] [Assertion EPred] [WP m Pred EPred] (x : OptionT m α)
+theorem orElse_OptionT_wp [Monad m] [Assertion Pred] [Assertion EPred] [WPMonad m Pred EPred] (x : OptionT m α)
     (h : Unit → OptionT m α) :
   wp x post ⟨wp (h ()) post epost, epost.tail⟩ ⊑
     wp (OrElse.orElse x h : OptionT m α) post epost := by
   simp only [wp, OrElse.orElse, OptionT.run]
-  apply PartialOrder.rel_trans; rotate_left; apply WP.wp_bind
-  apply WP.wp_consequence (m := m); intro o; cases o with
+  apply PartialOrder.rel_trans; rotate_left; apply WPMonad.wp_bind
+  apply WPMonad.wp_consequence (m := m); intro o; cases o with
   | some a =>
-    apply PartialOrder.rel_trans; rotate_left; apply WP.wp_pure
+    apply PartialOrder.rel_trans; rotate_left; apply WPMonad.wp_pure
     simp [EPost.cons.pushOption]; exact PartialOrder.rel_refl
   | none => exact PartialOrder.rel_refl
 
-end Std.Experimental.Do.WP
+end Std.Experimental.Do.WPMonad
